completed multi-step energy error bound

leapfrog_project/lf_harm_theorems.v
@@ -1,6 +1,6 @@
 From Flocq Require Import Binary Bits Core.
 From compcert.lib Require Import IEEE754_extra Coqlib Floats Zbits Integers.
-Require Import vcfloat float_lib lf_harm_float lf_harm_real lf_harm_lemmas.
+Require Import vcfloat float_lib lf_harm_float lf_harm_real optimize real_lemmas lf_harm_lemmas.
 Set Bullet Behavior "Strict Subproofs". 
 
 Import FPLangOpt. 
@@ -10,11 +10,13 @@ Import Test.
 
 Import Interval.Tactic.
 
-
-Definition error_v := (5079915575529618 / 75557863725914323419136)%R.
+(* these defs are pulled from bounds proofs in lf_harm_lemmas *)
+Definition error_v := (5079915575529842 / 75557863725914323419136)%R.
 (* error_v = 6.723212283974809e-08 *)
-Definition error_x := (4716905030025237 / 37778931862957161709568)%R.
+Definition error_x := (4716905030025348 / 37778931862957161709568)%R.
 (* error_x = 1.2485543654690345e-07*)
+Definition one_step_sum_bnd_x := (4646536420130942 / 2251799813685248)%R.
+Definition one_step_sum_bnd_v := (4646570650113373 / 2251799813685248)%R.
 
 
 (* single step position error *)
@@ -26,62 +28,12 @@ Theorem one_step_error_x:
          error_x.
 Proof.
 intros.
-set (bmap:= leapfrog_bmap) in *.
-hnf in bmap. simpl in bmap.
-match goal with |- context [ rval ?env ?e] =>
-simplify_shift_div_opt e
-end.
-(*unfold x'.*)
-match goal with |- context [ rval ?env ?e] =>
-get_rndval_with_conds e
-end.
-(* introduce and prove validity conditions *)
-(* for optmize_div x', there are 4 conditions *) 
-+ get_conds2;
-repeat (apply List.Forall_cons; try apply List.Forall_nil;
-try solve_one_cond2; 
-try interval).
-+ match goal with |- context [ rval ?env ?e] =>
-get_rndval_with_cond_correct e H0 H1 rndval s p;
-set (ty:= type_of_expr e) in *;
-simpl in ty;
-cbv [Datatypes.id] in ty;   
-repeat change (type_lub Tsingle Tsingle) with Tsingle in ty; 
-unfold ty in *; clear ty
-end.
-(* Populate hyps with some bounds on x and v*)
-fv_prepare_assumptions.
-(* turn rndval rexp to flt with eps delt *)
-rndval_replace.
-subst si2 s r;
-get_eps_delts.
-clear correct rndval H0 H1 H2 H3 e m H7.
-revert e0. reduce_abs_error. 
-(* env rewrite *)
-replace ((env_ (leapfrog_vmap val_x val_v))) 
-  with (leapfrog_env 
-  val_x val_v) in * by
-(apply lf_env_eq; apply BMD).
-(* var rewrites *)
-replace (leapfrog_env val_x val_v Tsingle lf_harm_lemmas._x) with 
-  val_x in * by 
-  (cbv in Hval_x;inversion Hval_x; clear Hval_x; subst; auto).
-replace (leapfrog_env 
-  val_x val_v Tsingle lf_harm_lemmas._v) with val_v in * by 
-(cbv in Hval_v;inversion Hval_v; clear Hval_v; subst; auto).
-change (fprec Tsingle) with 24%Z in *; 
-change (femax Tsingle) with 128%Z in *.
-
-intros. rewrite <- e0; clear H e0.
-
-match goal with |- context [Rabs (?v) <= _] =>
-field_simplify v
-end.
-
-match goal with |- context [Rabs (?v) <= _] =>
-interval_intro (Rabs v)
-end.
-unfold error_x;  nra.
+unfold error_x.
+(destruct (rndval_with_cond O (mempty  (Tsingle, Normal)) (optimize_div x')) 
+  as [[r [si2 s]] p] eqn:rndval).
+pose proof (rndval_with_cond_correct_optx x v H r si2 s p rndval)
+  as rndval_result. 
+intro_absolute_error_bound Tsingle Normal H x v rndval_result.
 Qed.
 
 
@@ -94,61 +46,83 @@ Theorem one_step_error_v:
          error_v.
 Proof.
 intros.
-set (bmap:= leapfrog_bmap) in *.
-hnf in bmap. simpl in bmap.
-match goal with |- context [ rval ?env ?e] =>
-simplify_shift_div_opt e
-end.
-match goal with |- context [ rval ?env ?e] =>
-get_rndval_with_conds e
-end.
-(* introduce and prove validity conditions *)
-(* for optmize_div v', there are 7 conditions *) 
-+ get_conds2;
- repeat (apply List.Forall_cons; try apply List.Forall_nil;
-try solve_one_cond2; 
-try interval).
-+ match goal with |- context [ rval ?env ?e] =>
-get_rndval_with_cond_correct e H0 H1 rndval s p;
-set (ty:= type_of_expr e) in *;
-simpl in ty;
-cbv [Datatypes.id] in ty;   
-repeat change (type_lub Tsingle Tsingle) with Tsingle in ty; 
-unfold ty in *; clear ty
-end.
-(* Populate hyps with some bounds on x and v*)
-fv_prepare_assumptions.
-(* turn rndval rexp to flt with eps delt *)
-rndval_replace.
-subst si2 s r;
-get_eps_delts.
-clear correct rndval H0 H1 H2 H3 e m H7.
-revert e0. reduce_abs_error. 
-(* env rewrite *)
-replace ((env_ (leapfrog_vmap val_x val_v))) 
-  with (leapfrog_env 
-  val_x val_v) in * by
-(apply lf_env_eq; apply BMD).
-(* var rewrites *)
-replace (leapfrog_env val_x val_v Tsingle lf_harm_lemmas._x) with 
-  val_x in * by 
-  (cbv in Hval_x;inversion Hval_x; clear Hval_x; subst; auto).
-replace (leapfrog_env 
-  val_x val_v Tsingle lf_harm_lemmas._v) with val_v in * by 
-(cbv in Hval_v;inversion Hval_v; clear Hval_v; subst; auto).
-change (fprec Tsingle) with 24%Z in *; 
-change (femax Tsingle) with 128%Z in *.
+unfold error_v.
+(destruct (rndval_with_cond O (mempty  (Tsingle, Normal)) (optimize_div v')) 
+  as [[r [si2 s]] p] eqn:rndval).
+pose proof (rndval_with_cond_correct_optv x v H r si2 s p rndval)
+  as rndval_result. 
+intro_absolute_error_bound Tsingle Normal H x v rndval_result.
+Qed.
 
-intros. rewrite <- e0; clear H e0.
-
-match goal with |- context [Rabs (?v) <= _] =>
-field_simplify (v)
+Lemma iter_real_bnded_x_v: forall x v : float32, 
+  (forall m: nat, 
+  forall x' v' : float32, 
+  (x',v') = (iternF m x%F32 v%F32) -> 
+  boundsmap_denote leapfrog_bmap (leapfrog_vmap x' v')) ->
+  forall x1 v1 : R,
+  x1 = B2R _ _ x ->
+  v1 = B2R _ _ v -> 
+forall n : nat,
+let bnd:= (1 + lf_harm_real.h - 1/2 * lf_harm_real.h^2) in
+  Rabs (fst(iternR n x1%R v1%R)) <= 
+powerRZ bnd (Z.of_nat n) /\
+  Rabs (snd(iternR n x1%R v1%R)) <= 
+powerRZ bnd (Z.of_nat n).
+Proof.
+intros.
+induction n.
++ simpl.
+pose proof H 0%nat x v. unfold iternF, leapfrog' in H2.
+pose proof H2 eq_refl.
+fvs_from_bndsmap_hyp H3;
+lf_rewrites;
+split.
+all: (apply Rbasic_fun.Rabs_le; nra).
++ assert (bnd <> 0) as Hbnd by (unfold bnd, lf_harm_real.h; nra).
+replace (Z.of_nat (S n)) with ( (Z.of_nat n + 1%Z)%Z) by lia. 
+rewrite ?powerRZ_add; auto. rewrite ?powerRZ_1.
+rewrite ?step_iternR.
+destruct (iternR n x1 v1) as (xnr, vnr). 
+unfold iternR, leapfrog_stepR, fst, snd, lf_harm_real.h, lf_harm_real.F in *.
+match goal with |- Rabs(?a) <= _ /\ Rabs(?b) <= _ =>
+field_simplify b ;
+field_simplify a 
 end.
-
-match goal with |- context [Rabs (?v) <= _] =>
-interval_intro (Rabs v)
-end.
-unfold error_v; nra.
+split; destruct IHn.
+- rewrite Rcomplements.Rabs_div; try nra.
+rewrite Rcomplements.Rle_div_l; try (apply Rabs_pos_lt; nra).
+eapply Rle_trans.
+eapply Rabs_triang.
+rewrite ?abs_mul; try interval; try nra.
+eapply Rle_trans.
+eapply Rplus_le_compat.
+eapply Rmult_le_compat_l in H2. apply H2. nra.
+eapply Rmult_le_compat_l in H3. apply H3. nra.
+rewrite <- Rmult_plus_distr_r .
+rewrite Rmult_comm.
+rewrite Rmult_assoc.
+eapply Rmult_le_compat_l. 
+apply powerRZ_le; unfold bnd; nra.
+unfold bnd; field_simplify. 
+rewrite Rabs_pos_eq; nra.
+- rewrite Rcomplements.Rabs_div; try nra.
+rewrite Rcomplements.Rle_div_l; try (apply Rabs_pos_lt; nra).
+eapply Rle_trans.
+replace ((4192256 * vnr - 131040 * xnr) ) with
+(4192256 * vnr + 131040 * -xnr) by nra. 
+eapply Rabs_triang.
+rewrite ?abs_mul; try interval; try nra.
+eapply Rle_trans.
+eapply Rplus_le_compat.
+eapply Rmult_le_compat_l in H3. apply H3. nra. 
+rewrite Rabs_Ropp. eapply Rmult_le_compat_l in H2. apply H2. nra.
+rewrite <- Rmult_plus_distr_r .
+replace (powerRZ bnd (Z.of_nat n) * bnd * Rabs 4194304) with
+(powerRZ bnd (Z.of_nat n) * (bnd * Rabs 4194304)) by nra.
+rewrite Rmult_comm.
+eapply Rmult_le_compat_l.
+apply powerRZ_le; unfold bnd; nra.
+unfold bnd. field_simplify. interval.
 Qed.
 
 
@@ -178,6 +152,7 @@ apply binary_float_eqb_eq in H2; subst; reflexivity.
 + rewrite (@env_rval_reify_correct_leapfrog_stepx x v x1 v1); auto.
 Qed.
 
+
 Lemma local_error_v:
   forall x v : float32,
   forall x1 v1 : R,
@@ -202,6 +177,22 @@ generalize (fval (leapfrog_env x v) (optimize_div v'));
 rewrite optimize_div_type; intros;
 apply binary_float_eqb_eq in H2; subst; reflexivity.
 + rewrite (@env_rval_reify_correct_leapfrog_stepv x v x1 v1); auto.
+Qed.
+
+
+Lemma local_error_v_2 :
+  forall x v : float32,
+  boundsmap_denote leapfrog_bmap (leapfrog_vmap x v)-> 
+  Rabs (B2R _ _ (fval (leapfrog_env  x v) (optimize_div v')))
+   <= error_v + Rabs (rval (leapfrog_env  x v) (optimize_div v'))  .
+Proof.
+intros.
+pose proof one_step_error_v x v H.
+apply Rabs_le_minus. 
+match goal with |- context [ Rabs(?a - ?b) <= _ ] =>
+replace (Rabs(a - b)) with (Rabs(b -a)) by (apply Rabs_minus_sym)
+end.
+apply one_step_error_v; auto. 
 Qed.
 
 Lemma global_error_x_aux : 
@@ -332,19 +323,75 @@ try interval with
 (i_bisect (INR n), i_depth 15).
 Qed.
 
+
+Definition global_error_val n := 
+(2*(pow lf_harm_real.h 3) * sqrt (INR n))%R.
+
+
+Definition iter_R_val := 
+(1 + lf_harm_real.h - 1/2 * lf_harm_real.h^2).
+
+
+Lemma global_error_corollary:
+forall x v : float32, 
+  (forall m: nat, 
+  forall x' v' : float32, 
+  (x',v') = (iternF m x%F32 v%F32) -> 
+  boundsmap_denote leapfrog_bmap (leapfrog_vmap x' v')) ->
+  forall n: nat, 
+  forall x1 v1 : R,
+  x1 = B2R _ _ x ->
+  v1 = B2R _ _ v -> 
+  INR n <= 0.5 * 1/lf_harm_real.h -> 
+  Rabs (fst(iternR n x1%R v1%R) + B2R 24 128 (fst (iternF n x v))) <= 
+ 2 * Rabs (fst(iternR n x1%R v1%R)) + global_error_val n
+ /\
+  Rabs (snd(iternR n x1%R v1%R) + B2R 24 128 (snd (iternF n x v))) <= 
+ 2 * Rabs (snd(iternR n x1%R v1%R)) + global_error_val n.
+Proof.
+intros.
+pose proof global_error x v H n x1 v1 H0 H1 H2.
+destruct H3.
+split.
++ eapply Rle_trans.
+eapply Rabs_triang.
+match goal with |- context [_ <= 2 * ?a + ?b ] =>
+replace (2 *a + b) with (a + (a + b)) by nra 
+end.
+eapply  Rplus_le_compat_l .
+rewrite Rplus_comm.
+eapply Rabs_le_minus.
+rewrite <- Rabs_Ropp.
+rewrite Ropp_minus_distr.
+apply H3.
++ eapply Rle_trans.
+eapply Rabs_triang.
+match goal with |- context [_ <= 2 * ?a + ?b ] =>
+replace (2 *a + b) with (a + (a + b)) by nra 
+end.
+eapply  Rplus_le_compat_l .
+rewrite Rplus_comm.
+eapply Rabs_le_minus.
+rewrite <- Rabs_Ropp.
+rewrite Ropp_minus_distr.
+apply H4.
+Qed.
+
+
 Definition H_osc (x v :R) : R := x^ 2 + v^2. 
 
-Lemma local_energy_error: 
+
+Theorem local_energy_error: 
   forall x v : float32,
     boundsmap_denote (leapfrog_bmap ) (leapfrog_vmap x v)->
     let xf2r := (B2R _ _ (fval (leapfrog_env  x v) (optimize_div x'))) in
     let vf2r := (B2R _ _ (fval (leapfrog_env  x v) (optimize_div v'))) in
     let xr := rval (leapfrog_env  x v) (optimize_div x') in
     let vr := rval (leapfrog_env  x v) (optimize_div v') in
-    Rabs (H_osc xr vr - H_osc xf2r vf2r) <=  
-(5737052551188771447961625990175617189626654515220295204472916317044736 /
-     14474011154664524427946373126085988481658748083205070504932198000989141204992).
-(* 3.96369223e-7 *)
+    Rabs (H_osc xr vr - H_osc xf2r vf2r) <= 
+5737052551189115355431825195770061827073493817295873037556855259267072 /
+     14474011154664524427946373126085988481658748083205070504932198000989141204992.
+(*3.963692227320304e-07*)
 Proof.
 intros.
 set (bmap:= leapfrog_bmap) in *.
@@ -362,10 +409,103 @@ match goal with
   |- context [ Rabs (?a) * Rabs (?b) + Rabs (?c) *Rabs (?d) <= _] =>
 pose proof Rabs_le_aux 
   a b c d 
-  (4646536420130843 / 2251799813685248) error_x (4646570650113169 / 2251799813685248) error_v
+  one_step_sum_bnd_x error_x one_step_sum_bnd_v error_v
   H2 H0 H3 H1
 end.
-unfold error_x, error_v in *.
+unfold error_x, error_v, one_step_sum_bnd_v, one_step_sum_bnd_x in *.
 field_simplify in H4.
 nra. 
+Qed.
+
+
+Theorem global_energy_error: 
+  forall x v : float32,
+(forall m: nat, 
+  forall x' v' : float32, 
+  (x',v') = (iternF m x%F32 v%F32) -> 
+  boundsmap_denote leapfrog_bmap (leapfrog_vmap x' v')) ->
+  forall n: nat, 
+  forall x1 v1 : R,
+  x1 = B2R _ _ x ->
+  v1 = B2R _ _ v -> 
+  INR n <= 0.5 * 1/lf_harm_real.h -> 
+    let xf2r := B2R _ _ (fst(iternF n x%F32 v%F32)) in
+    let vf2r := B2R _ _ (snd(iternF n x%F32 v%F32)) in
+    let xr := fst(iternR n x1%R v1%R) in
+    let vr := snd(iternR n x1%R v1%R) in
+    
+    Rabs (H_osc xr vr - H_osc xf2r vf2r) <= 
+    (4 * powerRZ iter_R_val (Z.of_nat n) * global_error_val n +
+2 * global_error_val n ^ 2)%R.
+Proof.
+intros. 
+
+unfold H_osc.
+eapply Rle_trans.
+eapply Rabs_triang_aux4.
+
+pose proof global_error_corollary x v H n x1 v1 H0 H1 H2; destruct H3.
+pose proof global_error x v H n x1 v1 H0 H1 H2; destruct H5.
+
+eapply  Rle_trans.
+eapply Rplus_le_compat_l.
+eapply Rmult_le_compat_r; try interval.
+apply H4.
+
+eapply  Rle_trans.
+eapply Rplus_le_compat_l.
+eapply Rmult_le_compat_l.
+unfold global_error_val.
+unfold lf_harm_real.h.  
+eapply Rplus_le_le_0_compat. 
+eapply Rmult_le_pos; try nra.
+apply Rabs_pos. 
+eapply Rmult_le_pos; try nra.
+apply sqrt_positivity. 
+apply pos_INR.
+apply H6.
+
+eapply  Rle_trans.
+eapply Rplus_le_compat_r.
+eapply Rmult_le_compat_l; try interval.
+apply H5.
+
+eapply  Rle_trans.
+eapply Rplus_le_compat_r.
+eapply Rmult_le_compat_r.
+eapply Rmult_le_pos; unfold lf_harm_real.h; try nra.
+apply sqrt_positivity. 
+apply pos_INR.
+apply H3.
+
+pose proof H n.
+destruct (iternF n x v). simpl in xf2r. simpl in vf2r.
+pose proof H7 f f0 eq_refl.
+pose proof iter_real_bnded_x_v x v H x1 v1 H0 H1 n.
+destruct H9.
+fold iter_R_val in *.
+
+eapply  Rle_trans.
+eapply Rplus_le_compat_r.
+eapply Rmult_le_compat_r.
+eapply Rmult_le_pos; try nra; try unfold lf_harm_real.h; try nra.  
+apply sqrt_positivity. 
+apply pos_INR.
+eapply Rplus_le_compat_r.
+eapply Rmult_le_compat_l; try nra.
+apply H9.
+
+eapply  Rle_trans.
+eapply Rplus_le_compat_l.
+eapply Rmult_le_compat_r.
+eapply Rmult_le_pos; try nra; try unfold lf_harm_real.h; try nra.  
+apply sqrt_positivity. 
+apply pos_INR.
+eapply Rplus_le_compat_r.
+eapply Rmult_le_compat_l; try nra.
+apply H10.
+
+fold (global_error_val n).
+field_simplify.
+nra.
 Qed.
